WIP

ems/ModSemE.v
@@ -128,9 +128,10 @@ Section EVENTS.
   (*** use dummy mname? ***)
   (* Definition FPut E `{rE -< E} (mn: mname) (fr: GRA): itree E unit := *)
 
-  Definition Es: Type -> Type := ((callE +' pE) +' eventE).
-  Definition Es': Type -> Type := (callE +' (pE +' eventE)).
-  Definition prf: Es -< Es' := (ReSum_sum IFun sum1 (callE +' pE) eventE Es').
+  Definition Es: Type -> Type := (callE +' (pE +' eventE)).
+  (* Definition Es: Type -> Type := ((callE +' pE) +' eventE). *)
+  (* Definition Es': Type -> Type := (callE +' (pE +' eventE)). *)
+  (* Definition prf: Es -< Es' := (ReSum_sum IFun sum1 (callE +' pE) eventE Es'). *)
 
   (* Inductive mdE: Type -> Type := *)
   (* | MPut (mn: mname) (r: GRA): mdE unit *)
@@ -167,9 +168,7 @@ Section EVENTS.
   (*   interp_pE (interp_rE (interp_mrec prog itr0) rst0) pst0 *)
   (* . *)
   Definition interp_Es A (prog: callE ~> itree Es) (itr0: itree Es A) (st0: p_state): itree (void1 +' eventE) (p_state * _)%type :=
-    let prog': callE ~> itree Es' := (fun _ ce => resum_itr (H:=prf) (prog _ ce)) in
-    let itr0': itree Es' A := resum_itr (H:=prf) itr0 in
-    '(st1, v) <- interp_pE (interp_mrec prog' itr0') st0;;
+    '(st1, v) <- interp_pE (interp_mrec prog itr0) st0;;
     Ret (st1, v)
   .
   
@@ -195,18 +194,18 @@ Section EVENTS.
   .
 
   Global Program Instance itree_Bar {R}: Bar (itree Es R) :=
-    fun itr => interp (case_ (case_ trivial_Handler core_h) trivial_Handler) itr
+    fun itr => interp (case_ trivial_Handler (case_ core_h trivial_Handler)) itr
   .
   Global Program Instance ktree_Bar {R S}: Bar (ktree Es R S) := fun ktr x => |ktr x|.
 
   Definition focus_left: itree Es ~> itree Es :=
     fun _ itr =>
-      interp (case_ (case_ trivial_Handler focus_left_h) trivial_Handler) itr
+      interp (case_ trivial_Handler (case_ focus_left_h trivial_Handler)) itr
   .
 
   Definition focus_right: itree Es ~> itree Es :=
     fun _ itr =>
-      interp (case_ (case_ trivial_Handler focus_right_h) trivial_Handler) itr
+      interp (case_ trivial_Handler (case_ focus_right_h trivial_Handler)) itr
   .
 
 
