ems/Skeleton.v
@@ -8,6 +8,7 @@ Set Implicit Arguments.
 Local Open Scope nat_scope.
 
 Notation gname := string (only parsing). (*** convention: not capitalized ***)
+Notation mname := string (only parsing). (*** convention: capitalized ***)
 
 
 
